DecodeTape now works in larger alphabet

theories/TM/Single/DecodeTapes.v
@@ -1,55 +1,30 @@
 From Undecidability.TM Require Import TM ProgrammingTools Code.Decode.
 
 From Undecidability.TM Require Single.EncodeTapes Single.StepTM Single.EncodeTapesInvariants CaseList.
-Require Import FunInd Lia Ring Arith.
+Require Import FunInd Lia Ring Arith Program.Wf.
 
-From Coq.ssr Require Import ssrfun.
+From Coq.ssr Require ssrfun.
+Module Option := ssrfun.Option.
+
 Module CheckEncodesTape.
   Section checkEncodesTape.
 
     Import EncodeTapes StateWhile CaseList Mono Multi MoveToSymbol Copy Switch If Combinators Single.EncodeTapesInvariants.
     
-    Context (sig:finType) (n:nat).
+    Context (sig : Type) (tau:finType) (n:nat) {I : Retract (sigTape sig) tau}.
+
+    Remove Hints Retract_id : typeclass_instances.
     
-    Notation sig__M := (FinType(EqType(sigTape sig))).
+    Notation sig__M := (sigTape sig).
 
-    Definition Rel : pRel sig__M bool 1 := ContainsEncoding.Rel (encode_tape (sig:=sig)).
+    Definition Rel : pRel tau bool 1 := ContainsEncoding.Rel (Encode_tape sig) Retr_f.
 
-    Definition M2 x :pTM sig__M bool 1 := if negb (Option.apply (@isMarked sig) false x)
-                                 then Return Nop false
-                                 else
-                                   MoveToSymbol (fun x => isMarked x || isLeftBlank x || isRightBlank x || isNilBlank x) id;;
-                                   Relabel ReadChar (Option.apply isRightBlank false).
-
-    Definition f__M2 x t : (bool*tape sig__M) :=
-      if negb (Option.apply (@isMarked sig) false x)
-      then (false,t)
-      else let t' := MoveToSymbol_Fun (fun x => isMarked x || isLeftBlank x || isRightBlank x) id t in
-           (Option.apply isRightBlank false (current t'),t').
-
-    Definition caseFirstSymbol : pTM sig__M (bool+bool) 1:=
-      Switch
-        ReadChar
-        (fun x =>
-           match x with
-             Some NilBlank => Return Nop (inl true)
-           | Some (LeftBlank b) => Return Nop (inr b)
-           | _ => Return Nop (inl false)
-           end).
-
-    Definition f__caseFirstSymbol (t: tape sig__M): (bool+bool):=
-      match current t with
-        Some NilBlank => inl true
-      | Some (LeftBlank b) => inr b
-      | _ => inl false
-      end.
-
-    Definition M__step : bool*bool -> pTM sig__M ((bool*bool) + bool) 1 :=
+    Definition M__step : bool*bool -> pTM tau ((bool*bool) + bool) 1 :=
       fun '(haveSeenMark,haveSeenSymbol) =>
         Switch
           ReadChar
           (fun x =>
-             match x with
+             match Option.bind Retr_g x with
                None => Return Nop (inr false)
              | Some c =>
                if (isMarked c && haveSeenMark) || isNilBlank c || isLeftBlank c || isRightBlank c
@@ -57,9 +32,9 @@ Module CheckEncodesTape.
                else Return (Move R) (inl (haveSeenMark || isMarked c,haveSeenSymbol || isSymbol c))
              end).
 
-    Definition f__step bs t : (bool * bool + bool) * tape sig__M :=
+    Definition f__step bs t : (bool * bool + bool) * tape tau :=
       let (haveSeenMark,haveSeenSymbol) := (fst bs,snd bs) in
-      match current t with
+      match Option.bind Retr_g (current t) with
         None => (inr false,t)
       | Some c =>
         if (isMarked c && haveSeenMark) || isNilBlank c || isLeftBlank c || isRightBlank c
@@ -70,27 +45,44 @@ Module CheckEncodesTape.
     Definition M' (bs : bool*bool) := 
       StateWhile M__step bs.
 
-    Function f' bs t { measure rlength t } : (bool * tape sig__M)  :=
+    (* Program Fixpoint f' bs (t : tape tau) { measure (rlength t) } : (bool * tape tau)  :=
+      let r := f__step bs t in
+      match fst r with 
+        inl bs' => f' bs' (snd r)
+      | inr b => (b,(snd r))
+      end.
+    Local Obligation Tactic := idtac.
+    Next Obligation. cbn.
+      intros [haveSeenMark haveSeenSymbol] [ | | | ? c' t__R] _ ?;cbn.
+      1-3:now intros [=].
+      destruct (Retr_g c') as [ c | ]. 2:now intros [= <-].
+      destruct c as [ [] | [] | | | ];cbn. all:try solve [inversion 1].
+      1-4:destruct haveSeenMark;cbn.
+      all:intros [= ->]. all:destruct t__R;cbn. all:nia.
+    Qed. *)
+    
+    Function f' bs (t : tape tau) { measure rlength t } : (bool * tape tau)  :=
       let r := f__step bs t in
       match fst r with 
         inl bs' => f' bs' (snd r)
       | inr b => (b,(snd r))
       end.
     Proof.
-      unfold f__step. intros [haveSeenMark haveSeenSymbol] [ | | | ? c t__R] ?;cbn.
+      unfold f__step. intros [haveSeenMark haveSeenSymbol] [ | | | ? c' t__R] ?;cbn.
       1-3:now intros [=].
+      destruct (Retr_g c') as [ c | ]. 2:now intros [= <-].
       destruct c as [ [] | [] | | | ];cbn. all:try solve [inversion 1].
       1-4:destruct haveSeenMark;cbn.
       all:intros [= <-]. all:destruct t__R;cbn. all:nia.
     Qed.
     
-    Definition M : pTM sig__M bool 1:=
-      If (Relabel ReadChar (Option.apply isLeftBlank false))
-         (Switch ReadChar (fun c => Move R;; M' (Option.apply (@isMarked _) false c,false)))
-         (Relabel ReadChar (Option.apply isNilBlank false)).
+    Definition M : pTM tau bool 1:=
+      If (Relabel ReadChar (fun c => Option.apply isLeftBlank false (Option.bind Retr_g c)))
+         (Switch ReadChar (fun c => Move R;; M' (Option.apply (@isMarked _) false (Option.bind Retr_g c),false)))
+         (Relabel ReadChar (fun c => Option.apply isNilBlank false (Option.bind Retr_g c))).
 
-    Definition f (t : tape sig__M) : (bool*tape sig__M) :=
-      match current t with
+    Definition f (t : tape tau) : (bool*tape tau) :=
+      match Option.bind Retr_g (current t) with
         None => (false,t)
       | Some c =>
         if isLeftBlank c then  f' (isMarked c,false) (tape_move_right t)
@@ -98,13 +90,6 @@ Module CheckEncodesTape.
       end.
 
     (** Verification*)
-
-
-    Local Arguments Vector.to_list {A n} (!v).
-
-    Local Arguments plus : simpl never.
-    Local Arguments mult : simpl never.
-    Local Arguments caseFirstSymbol : simpl never.
 
     Tactic Notation "destruct" "_" "in" constr(H):=
       match type of H with
@@ -130,7 +115,7 @@ Module CheckEncodesTape.
     Tactic Notation "destructBoth" constr(g) "as" simple_intropattern(P) :=
       match goal with
         |- (?REL _ ?R) =>
-        tacInEvar R (destruct g as P);destruct g as P;cbn zeta iota
+        tacInEvar R (destruct g as P);destruct g as P;cbn zeta iota beta
       end.
 
     
@@ -141,11 +126,11 @@ Module CheckEncodesTape.
     Proof.
       destruct bs as (seenMark, seenSymbol). eapply Realise_monotone.
       { unfold M__step;cbn. apply Switch_Realise. now TM_Correct.
-        introsSwitch c. destructBoth c as [c | ]. 2:now TM_Correct.
+        introsSwitch c'. destructBoth (Option.bind Retr_g c') as [c | ]. 2:now TM_Correct.
         destructBoth (isMarked c && seenMark || isNilBlank c || isLeftBlank c || isRightBlank c). all:TM_Correct.
       }
       hnf;cbn. intros t (y&t') (?&?&[-> -> ]&H);revert H.
-      destruct current. 2:{ cbn. now intros (->&_&->). }
+      destruct Option.bind. 2:{ cbn. now intros (->&_&->). }
       destruct _. all:cbn. all:intros (->&_&->). all:easy.
     Qed.
 
@@ -157,11 +142,11 @@ Module CheckEncodesTape.
     Proof.
       destruct bs as (seenMark, seenSymbol). eapply TerminatesIn_monotone.
       { unfold M__step;cbn. apply Switch_TerminatesIn. 1,2:now TM_Correct.
-        introsSwitch c. destructBoth c as [c | ]. 2:now TM_Correct.
+        introsSwitch c'. destructBoth (Option.bind Retr_g c') as [c | ]. 2:now TM_Correct.
         destructBoth (isMarked c && seenMark || isNilBlank c || isLeftBlank c || isRightBlank c). all:TM_Correct.
       }
       hnf;cbn. intros t y Hy. infTer 3. rewrite <- Hy.
-      2:{ intros ? ? [-> ->]. destruct current. 2:lia. destruct _. 2:reflexivity. nia. }
+      2:{ intros ? ? [-> ->]. destruct Option.bind. 2:lia. destruct _. 2:reflexivity. nia. }
       nia.
     Qed.
     
@@ -173,9 +158,9 @@ Module CheckEncodesTape.
         cbn;intros c. TM_Correct_step. now TM_Correct.
         unfold M'.
         eapply Realise_monotone with
-            (R:= fun t '(y,t')=> f' (oapp (isMarked (sig:=eqType_X (type sig))) false c, false) t[@Fin0] = (y,t'[@Fin0])).
+            (R:= fun t '(y,t')=> f' (Option.apply (@isMarked _) false (Option.bind Retr_g c), false) t[@Fin0] = (y,t'[@Fin0])).
         { eapply StateWhile_Realise. now eapply Realises__step. }
-        generalize (oapp (isMarked (sig:=eqType_X (type sig))) false c, false) as bs. clear c.
+        generalize (Option.apply (@isMarked _) false (Option.bind Retr_g c), false) as bs. clear c.
         apply StateWhileInduction. all:cbn - [f__step].
         -intros t bs b' t'. rewrite f'_equation. intros ->. reflexivity. 
         -intros t bs bs' t' t'' v'. rewrite f'_equation with (t:=t[@Fin0]). intros -> <-. reflexivity.
@@ -184,15 +169,15 @@ Module CheckEncodesTape.
       intros t (y&t1) [H |H];revert H.
       all:intros (?&(?&H1&->&->)&H);revert H.
       -intros (?&?&[-> ->]&_&t2&Ht2&<-).
-       unfold f. destruct current. 2:now inv H1.
+       unfold f. destruct Option.bind . 2:now inv H1.
        cbn in H1. rewrite <- H1. cbn. congruence.
       -intros (?&->&->&->). unfold f.
-       destruct current. 2:easy.
+       destruct Option.bind . 2:easy.
        cbn in *. now rewrite <- H1. 
     Qed.
 
     
-    Definition Ter : tRel sig__M 1:=
+    Definition Ter : tRel tau 1:=
       fun t k => 4 * (| tape_local (tape_move_right t[@Fin0]) |) + 9 <= k.
 
     Lemma Terminates : projT1 M ↓ Ter.
@@ -207,7 +192,7 @@ Module CheckEncodesTape.
         evar (time : nat -> nat). [time]:intros n0.
         apply StateWhileCoInduction with (T:= fun _ t k => time (length (tape_local t[@Fin0])) +c0 <= k). all:cbn - [f__step].
         -intros l t k Hk. infTer 2. intros y' t'.
-         unfold f__step. destruct current eqn:Hc.
+         unfold f__step. destruct Option.bind eqn:Hc.
          2:{intros [= <- _]; rewrite <- Hk. enough (3 <= c0). now nia. shelve. }
          destruct _ eqn:Hs. all: intros [= <- Ht']. 1:{ enough (3 <= c0). now nia. shelve. }
          rewrite <- Ht'. infTer 2. rewrite <- Hk.
@@ -222,42 +207,46 @@ Module CheckEncodesTape.
       ring_simplify. hnf in HT. cbn in *. nia.
     Qed.
     
-    Lemma f'_spec (seenMark seenSymbol : bool) t__L' b t__L c t__R res:
+    Lemma f'_spec (seenMark seenSymbol b : bool) (c:tau) t__L' t__L t__R res:
       (length (filter (@isMarked _) (t__L'++[LeftBlank b])) = if seenMark then 1 else 0)
       -> (forall x, x el t__L' -> isSymbol x = true)
       -> reflect (t__L' <> []) seenSymbol
-      -> res =  f' (seenMark,seenSymbol) (midtape (t__L'++LeftBlank b::t__L) c t__R)
+      -> res =  f' (seenMark,seenSymbol) (midtape (map Retr_f (t__L'++[LeftBlank b])++t__L) c t__R)
       ->  if fst res then
-           exists (x:tape sig) (t__R1 t__R2 : list sig__M),
-             t__R = t__R1++t__R2
-             /\ encode_tape x = LeftBlank b :: rev t__L'++c::t__R1
-             /\ snd res = midtape (tail (rev t__R1++[c])++t__L'++LeftBlank b::t__L) (hd c (rev t__R1++[c])) t__R2
+           exists (x:tape sig) t__R1 (t__R2 : list tau) c',
+             t__R = map Retr_f t__R1++t__R2
+             /\ Some c' = Retr_g c
+             /\ encode_tape x = LeftBlank b :: rev t__L'++c'::t__R1
+             /\ snd res = midtape (tail (rev (map Retr_f t__R1)++[c])++map Retr_f (t__L'++[LeftBlank b])++t__L) (hd c (rev (map Retr_f t__R1)++[c])) t__R2
          else
-           forall x (t__R1 t__R2 : list sig__M),
-             t__R = t__R1++t__R2 -> 
-             encode_tape x <> LeftBlank b :: rev t__L'++c::t__R1.
+           forall x t__R1 (t__R2 : list tau) c',
+             t__R = map Retr_f t__R1++t__R2 ->
+             Some c' = Retr_g c ->
+             encode_tape x <> LeftBlank b :: rev t__L'++c'::t__R1.
     Proof.
+      rewrite map_app;cbn.
       remember (length t__R) as n0 eqn: Hn0. revert t__R Hn0 t__L' c res seenMark seenSymbol.
       induction n0 as [n0 IH] using lt_wf_ind. intros ? -> ? ? res ? ?;cbn in *.
       intros H__seenMark H__symbs H__seenSymbol Hres. 
-      rewrite f'_equation in Hres.
-      destruct c;cbn. 1-3:clear IH.
-      -replace (res.1) with false.
-       2:{ cbn in Hres. destruct marked;cbn in Hres. destruct seenMark in Hres;cbn in Hres. all:now subst. }
+      rewrite f'_equation in Hres. remember (f__step _ _) as f eqn:Hf. unfold f__step in Hf;cbn in Hf.
+      destruct (Retr_g c) as [ [] | ] eqn:Hgc ;cbn. 1-3,6:clear IH.
+      -replace (fst res) with false.
+       2:{ destruct marked;cbn in Hf. destruct seenMark in Hf;cbn in Hf. all:now subst. }
        clear - H__symbs.
-       intros ? ? ? -> (Hneq&Hsym&(?&Hlast)&_)%encode_tape_invariants_partial;cbn in *. 2:now setoid_rewrite <- in_rev.
+       intros ? ? ? ? -> [= ->] (Hneq&Hsym&(?&Hlast)&_)%encode_tape_invariants_partial;cbn in *. 2:now setoid_rewrite <- in_rev.
        destruct t__R1. easy. discriminate (Hsym (LeftBlank marked)). rewrite tl_app. 2:now length_not_eq. now eauto.     
-      -revert Hres. cbn. rewrite !orb_true_r.
+      -cbn in Hf. rewrite !orb_true_r in Hf. subst f. revert Hres. 
        destruct marked;cbn in *. destruct seenMark;cbn in *. all:intros ->;cbn. 3:destruct seenMark;cbn. 2,3:destruct seenSymbol;cbn.
-       +intros ? ? ? -> (Hneq&Hsym&(?&Hlast)&Hmarks)%encode_tape_invariants_partial;cbn in *. 2:now setoid_rewrite <- in_rev.
+       +intros ? ? ? ? -> [= ->] (Hneq&Hsym&(?&Hlast)&Hmarks)%encode_tape_invariants_partial;cbn in *. 2:now setoid_rewrite <- in_rev.
         autorewrite with list in *. nia.
        +edestruct invert_symbols_0_marked with (t:= t__L') as (t__R2&->).
         1,2:autorewrite with list in *. now nia. now intros;eapply H__symbs.
         destruct b. 1:{exfalso. autorewrite with list in H__seenMark. now cbn in H__seenMark;nia. } 
         destruct t__R2 as [ | c' cs] eqn:Htp. 1:{exfalso. inversion H__seenSymbol. easy. } 
-        eexists (rightof _ _),[],_. repeat eapply conj. 1,3:reflexivity. cbn.
+        eexists (rightof _ _),[],_,_. repeat eapply conj. 1,2,4:reflexivity. cbn.
         autorewrite with list;cbn.  setoid_rewrite <- map_rev with (l:=cs) at 2. easy.
-       +intros ? ? ? -> (Hneq&Hsym&(?&Hlast)&Hmarks&Hnempty)%encode_tape_invariants_partial;cbn in *. 2:now setoid_rewrite <- in_rev.
+       +intros ? ? ? ? -> [= ->] (Hneq&Hsym&(?&Hlast)&Hmarks&Hnempty)%encode_tape_invariants_partial;cbn in *.
+        2:now setoid_rewrite <- in_rev.
         destruct t__L'. all:inv H__seenSymbol. 2:now apply H. cbn in *;autorewrite with list in *.
         destruct t__R1. 2:{ ediscriminate (Hsym (RightBlank _)). rewrite tl_app. eauto. length_not_eq. }
         cbn in *. nia.
@@ -266,97 +255,111 @@ Module CheckEncodesTape.
          1,2:autorewrite with list in *;cbn in *. now nia. now intros;eapply H__symbs.
          destruct t__R2 eqn:?. 1:{exfalso. inversion H__seenSymbol. easy. }
          destruct (rev t__R2) eqn:Htp. 1:{exfalso. subst. revert Htp. length_not_eq. } 
-         eexists (leftof _ _),[],_. repeat eapply conj. 1,3:reflexivity. rewrite <- Heql. cbn.
-         autorewrite with list;cbn.  setoid_rewrite <- map_rev with (l:=t__R2). now rewrite Htp.
+         eexists (leftof _ _),[],_,_. repeat eapply conj. 1,2,4:reflexivity. rewrite <- Heql. cbn.
+         setoid_rewrite <- map_rev with (l:=t__R2). now rewrite Htp.
         *edestruct @invert_symbols_1_marked with (t:= t__L') as (?&?&?&->).
          1,2:autorewrite with list in *;cbn in *. now nia. now intros;eapply H__symbs.
-         eexists (midtape _ _ _),[],_. repeat eapply conj. 1,3:reflexivity. cbn.
+         eexists (midtape _ _ _),[],_,_. repeat eapply conj. 1,2,4:reflexivity. cbn.
          repeat (autorewrite with list;cbn).  setoid_rewrite map_rev. easy.
-       +intros ? ? ? -> (Hneq&Hsym&(?&Hlast)&Hmarks&?)%encode_tape_invariants_partial;cbn in *. 2:now setoid_rewrite <- in_rev.
+       +intros ? ? ? ? -> [= -> ] (Hneq&Hsym&(?&Hlast)&Hmarks&?)%encode_tape_invariants_partial;cbn in *.
+        2:now setoid_rewrite <- in_rev.
         destruct t__R1. 2:{ ediscriminate (Hsym (RightBlank _)). rewrite tl_app. 2:now length_not_eq. eauto. }
-        destruct t__L'. 2:{ inversion H__seenSymbol. now apply H0. }
+        destruct t__L'. 2:{ inversion H__seenSymbol. now apply H. }
         cbn in *. nia.
-       +intros ? ? ? -> (Hneq&Hsym&(?&Hlast)&Hmarks&?)%encode_tape_invariants_partial;cbn in *. 2:now setoid_rewrite <- in_rev.
+       +intros ? ? ? ? -> [= ->] (Hneq&Hsym&(?&Hlast)&Hmarks&?)%encode_tape_invariants_partial;cbn in *.
+        2:now setoid_rewrite <- in_rev.
         destruct t__R1. 2:{ ediscriminate (Hsym (RightBlank _)). rewrite tl_app. 2:now length_not_eq. eauto. }
         cbn in *. autorewrite with list in *. nia.
-      -replace (res.1) with false.
-       2:{ cbn in Hres. destruct seenMark in Hres;cbn in Hres. all:now subst. }
+      -replace (fst res) with false.
+       2:{ cbn in Hf. destruct seenMark in Hf;cbn in Hf. all:now subst. }
        clear - H__symbs.
-       intros ? ? ? -> (Hneq&Hsym&(?&Hlast)&_)%encode_tape_invariants_partial;cbn in *. 2:now setoid_rewrite <- in_rev.
+       intros ? ? ? ? -> [= -> ] (Hneq&Hsym&(?&Hlast)&_)%encode_tape_invariants_partial;cbn in *. 2:now setoid_rewrite <- in_rev.
        destruct t__R1. easy. discriminate (Hsym (NilBlank)). rewrite tl_app. 2:now length_not_eq. now eauto.   
-      -revert Hres. cbn. destruct seenMark;cbn.
-       {clear IH. intros ->;cbn.
-        intros ? ? ? -> (Hneq&Hsym&(?&Hlast)&?&?)%encode_tape_invariants_partial;cbn in *. 2:now setoid_rewrite <- in_rev.
+      -subst f res;cbn. easy.
+      -revert Hf Hres. cbn. destruct seenMark;cbn.
+       {clear IH. intros -> ->;cbn.
+        intros ? ? ? ? -> [= ->](Hneq&Hsym&(?&Hlast)&?&?)%encode_tape_invariants_partial;cbn in *. 2:now setoid_rewrite <- in_rev.
         cbn in *. autorewrite with list in *. nia.
-       }
+       } intros ->;cbn.
        destruct t__R.
        { clear IH. cbn. rewrite f'_equation;cbn.  
          intros ->;cbn.
-         intros ? ? ? Hnil (Hneq&Hsym&(?&Hlast)&?&?)%encode_tape_invariants_partial;cbn in *. 2:now setoid_rewrite <- in_rev.
+         intros ? ? ? ? Hnil [= ->] (Hneq&Hsym&(?&Hlast)&?&?)%encode_tape_invariants_partial;cbn in *.
+         2:now setoid_rewrite <- in_rev.
          destruct t__R1. 2:easy. destruct t__R2. 2:easy. easy.
        }
        cbn. intros H.
        autorewrite with list in H__seenMark. destruct b;cbn in H__seenMark. now nia. 
-       specialize IH with (t__L' := MarkedSymbol s :: t__L');cbn in IH. pose (H' := H);eapply IH in H';clear IH.
+       specialize IH with (t__L' := MarkedSymbol s :: t__L');cbn in IH. erewrite <- !(retract_g_inv Hgc) in IH.
+       pose (H' := H);eapply IH in H';clear IH.
        3:reflexivity. 2:nia. 2:now autorewrite with list in *;nia. 2:now intros ? [<- | ];eauto.
        2:now rewrite orb_true_r;constructor.
        destruct res as [[] t'];cbn in *.
-       +destruct H' as (x&t__R1&t__R2&->&Hx&->).
-        eexists x,(s0::t__R1),t__R2.
-        repeat (cbn in Hx|-*;autorewrite with list in Hx|-* ). split. 2:split. 1,2:congruence.
-        destruct (rev t__R1);cbn;now autorewrite with list.
-       +intros x ? ? H__R Hx. specialize encode_tape_invariants_partial with (1:=Hx) as (Hneq&Hsym&(?&Hlast)&_);cbn in *. now setoid_rewrite <- in_rev.
+       +destruct H' as (x&t__R1&t__R2&c'&->&Hc'&Hx&->).
+        eexists x,(_::t__R1),t__R2,_.
+        repeat (cbn in Hx|-*;autorewrite with list in Hx|-* ). erewrite <- retract_g_inv. 2:symmetry;eassumption.
+        split. 2:split. 3:split.
+        1,2:reflexivity. easy.
+        destruct (rev (map f__I t__R1));cbn;now autorewrite with list.
+       +intros x ? ? ? H__R [= ->] Hx. specialize encode_tape_invariants_partial with (1:=Hx) as (Hneq&Hsym&(?&Hlast)&_);cbn in *. now setoid_rewrite <- in_rev.
         destruct (rev t__R1) eqn:Heq. all:inv Hlast.
-        destruct t__R1. now inv Heq. inv H__R. eapply H'. reflexivity.  rewrite Hx;cbn;autorewrite with list;cbn. reflexivity.
-      -revert Hres. cbn.
+        destruct t__R1. now inv Heq. inv H__R. eapply H'. reflexivity.  now rewrite retract_g_adjoint.
+        rewrite Hx;cbn;autorewrite with list;cbn. reflexivity.
+      -revert Hf Hres. cbn. intros ->;cbn.
        destruct t__R.
        { clear IH. cbn. rewrite f'_equation;cbn.  
          intros ->;cbn.
-         intros ? ? ? Hnil (Hneq&Hsym&(?&Hlast)&?&?)%encode_tape_invariants_partial;cbn in *. 2:now setoid_rewrite <- in_rev.
-         destruct t__R1. 2:easy. destruct t__R2. 2:easy. easy.
+         intros ? ? ? ? Hnil [= ->] (Hneq&Hsym&(?&Hlast)&?&?)%encode_tape_invariants_partial;cbn in *.
+         2:now setoid_rewrite <- in_rev.  destruct t__R1. 2:easy. destruct t__R2. 2:easy. easy.
        }
        cbn;intros H.
-       specialize IH with (t__L' := UnmarkedSymbol s :: t__L');cbn in IH. pose (H' := H);eapply IH in H';clear IH.
+       specialize IH with (t__L' := UnmarkedSymbol s :: t__L');cbn in IH. erewrite <- !(retract_g_inv Hgc) in IH.
+       pose (H' := H);eapply IH in H';clear IH.
        3:reflexivity. 2:lia. 3:now intros ? [<- | ];eauto. 3:now rewrite orb_true_r;constructor.
        2:{ autorewrite with list in *. destruct seenMark;cbn in *;nia. }
        destruct res as [[] t'];cbn in *.
-       +destruct H' as (x&t__R1&t__R2&->&Hx&->).
-        eexists x,(s0::t__R1),t__R2.
-        repeat (cbn in Hx|-*;autorewrite with list in Hx|-* ). split. 2:split. 1,2:congruence.
-        destruct (rev t__R1);cbn;now autorewrite with list.
-       +intros x ? ? H__R Hx. specialize encode_tape_invariants_partial with (1:=Hx) as (Hneq&Hsym&(?&Hlast)&_);cbn in *. now setoid_rewrite <- in_rev.
+       +destruct H' as (x&t__R1&t__R2&c'&->&Hc&Hx&->).
+        eexists x,(_::t__R1),t__R2,_. cbn.  erewrite <- retract_g_inv. 2:symmetry;eassumption.
+        repeat (cbn in Hx|-*;autorewrite with list in Hx|-* ). split. 2:split. 3:split. 1,2:reflexivity. easy.
+        destruct (rev (map f__I t__R1));cbn;now autorewrite with list.
+       +intros x ? ? ? H__R [= ->] Hx. specialize encode_tape_invariants_partial with (1:=Hx) as (Hneq&Hsym&(?&Hlast)&_);cbn in *. now setoid_rewrite <- in_rev.
         destruct (rev t__R1) eqn:Heq. all:inv Hlast.
-        destruct t__R1. now inv Heq. inv H__R. eapply H'. reflexivity.  rewrite Hx;cbn;autorewrite with list;cbn. reflexivity.
+        destruct t__R1. now inv Heq. inv H__R. eapply H'. 1:reflexivity. 1:now rewrite retract_g_adjoint. rewrite Hx;cbn;autorewrite with list;cbn. reflexivity.
     Qed.
 
     Lemma f_spec t b t':
       f t = (b,t')
       -> Rel [|t|] (b,[|t'|]).
     Proof.
-      unfold f;cbn. destruct current eqn:Hcur.
-      2:{ intros [= <- <-];cbn;intros ? ? ?. destruct x;cbn;eexists;(split;[reflexivity| ]). all:intros ->;inv Hcur. }
-      destruct t as [ | | | t__L s' t__R];inversion Hcur. subst s';clear Hcur.
+      unfold f;cbn. destruct Option.bind eqn:Hcur.
+      2:{ intros [= <- <-];cbn;intros ? ? ?. destruct x;cbn;eexists;(split;[reflexivity| ]).
+          all:intros ->;cbn in Hcur. all:rewrite retract_g_adjoint in Hcur;inv Hcur. }
+      destruct t as [ | | | t__L s' t__R];cbn in Hcur. all:inversion Hcur.
       destruct isLeftBlank eqn:H__LB.
       2:destruct isNilBlank eqn:H__NB.
-      2:{ intros [= <- <- ]. destruct s;inv H__NB. eexists (@niltape _),_,_;cbn. eauto 10. }
-      2:{ intros [= <- <- ]. intros ? x ?. destruct x;cbn;eexists;(split;[reflexivity | ]). all:destruct s;intros [= -> ->]. all:easy. }
+      2:{ intros [= <- <- ]. destruct s;inv H__NB. apply retract_g_inv in Hcur as ->. eexists (@niltape _),_,_;cbn. eauto 10. }
+      2:{ intros [= <- <- ]. intros ? x ?. destruct x;cbn;eexists;(split;[reflexivity | ]).
+          all:intros [=];subst. all:rewrite retract_g_adjoint in Hcur;inv Hcur. all:easy. }
       destruct s;inv H__LB.
-      destruct t__R. 1:{ cbn. rewrite f'_equation. cbn. intros [= <- <-]. intros ? x ?. destruct x;cbn;eexists;(split;[reflexivity | ]). all:intros [= -> ->]. all:revert H0. all:length_not_eq. }
-      intros H';symmetry in H'. assert (H:=H'). revert H. intros H%(f'_spec (t__L':=[])).
+      destruct t__R. 1:{ cbn. rewrite f'_equation. cbn. intros [= <- <-]. intros ? x ?. destruct x;cbn;eexists;(split;[reflexivity | ]). all:intros [= -> ->]. all:rewrite retract_g_adjoint in *;inv Hcur;inv H0.  all:revert H1. all:length_not_eq. }
+      intros H';symmetry in H'. assert (H:=H'). revert H. cbn. rewrite (retract_g_inv Hcur) at 1. intros H%(f'_spec (t__L':=[])).
       2:now destruct marked;cbn;nia. 2:easy. 2:now constructor. destruct b;cbn  in H.
-      -destruct H as (x&t__R1&t__R2&->&Hx&->). all:destruct (rev (encode_tape x)) eqn:Hlast.
-       1:{ rewrite Hx in Hlast. exfalso;revert Hlast; length_not_eq. }
-       do 4 eexists.
-       +rewrite Hx;cbn. eauto.
-       +setoid_rewrite Hlast at 1. rewrite Hx in Hlast. cbn in Hlast.
-        apply (f_equal (hd e)) in Hlast. cbn in Hlast. rewrite hd_app in Hlast. 2: length_not_eq. subst s.
-        rewrite Hx. cbn. rewrite <- !tl_app. 2,3:length_not_eq. repeat (autorewrite with list;cbn). eauto 10.
-      -intros ? x ?. exists (hd NilBlank (encode_tape x)). split. now destruct x.
-       intros [= <- H1 H2]. destruct encode_tape eqn:Heqt. now inv H1. cbn in *. subst s.
-       destruct l. 1:{ destruct x;cbn in Heqt;try now inv Heqt. all:revert Heqt. all:length_not_eq. }
-       inv H2. eapply H. 2:exact Heqt. reflexivity.
+      -destruct H as (x&t__R1&t__R2&c'&->&Hc&Hx&->). symmetry in Hc. erewrite (retract_g_inv Hc).
+       all:destruct (rev (encode_tape x)) eqn:Hlast.
+       1:{rewrite Hx in Hlast. exfalso;revert Hlast; length_not_eq. }
+       do 5 eexists.
+       +rewrite Hx;cbn. erewrite (retract_g_inv Hcur). auto.
+       +rewrite <- map_rev. setoid_rewrite Hlast at 1. rewrite Hx in Hlast. cbn in Hlast. split. easy.
+        apply (f_equal (map f__I)) in Hlast. apply (f_equal (hd (f__I c'))) in Hlast.
+        cbn in Hlast. rewrite map_app in Hlast. rewrite hd_app in Hlast. 2: length_not_eq.
+        autorewrite with list in Hlast. rewrite Hx. rewrite map_rev in *.
+        cbn. rewrite <- !tl_app. 2,3:length_not_eq. repeat (autorewrite with list in *;cbn in * ).
+        congruence.
+      -intros ? x ? . exists (f__I (hd NilBlank (encode_tape x))). split. now destruct x.
+       intros [= <- -> H2]. rewrite retract_g_adjoint in Hcur. inv Hcur. destruct encode_tape eqn:Heqt. now inv H3.
+       cbn in *. subst s. destruct l. 1:{ destruct x;cbn in Heqt;try now inv Heqt. all:revert Heqt. all:length_not_eq. }
+       inv H2. eapply H. 3:exact Heqt. reflexivity. now rewrite retract_g_adjoint.
     Qed.
-
 
   End checkEncodesTape.
 End CheckEncodesTape.
