theories/TM/Code/Decode.v
@@ -1,22 +1,23 @@
-From Undecidability.TM Require Import TM.
+From Undecidability.TM Require Import TM Code.
 
+Import Retracts.
 Module ContainsEncoding.
   Section containsEncoding.
     Local Unset Implicit Arguments.
 
-    Context {sig:Type} {n:nat} {X:Type}.
-    Context (encode : X -> list sig).
+    Context {sig tau:Type} {n:nat} {X:Type}.
+    Context (cX : codable sig X) (f : sig -> tau).
     (*Hypothesis (nonEmpty : forall x, encode x <> []).*)
 
-    Definition Rel : pRel sig bool 1 :=
+    Definition Rel : pRel tau bool 1 :=
       fun tin '(yout, tout) =>
         match yout with
           true => exists (x:X) t__L t__R,
-                 let t__x := encode x in
+                 let t__x := map f (encode x) in
                  (exists c__hd, hd_error t__x = Some c__hd /\  tin[@Fin0] = midtape t__L c__hd (tl t__x++t__R) )
                  /\ exists c__last, hd_error (rev t__x) = Some c__last /\ tout[@Fin0] = midtape (tl(rev t__x)++ t__L) c__last t__R
         | false => forall t__L (x:X) t__R,
-            let t__x := encode x in
+            let t__x := map f (encode x) in
             exists c__hd, hd_error t__x = Some c__hd /\
             tin[@Fin0] <> midtape t__L c__hd (tl t__x++t__R)
         end.
